LeanPy/Data/Addr.lean
@@ -1,0 +1,54 @@
+/-
+Copyright (c) 2025 Mac Malone. All rights reserved.
+Released under the Apache 2.0 license as described in the file LICENSE.
+Authors: Mac Malone
+-/
+
+namespace LeanPy
+
+/-- A runtime address. -/
+structure Addr where
+  private innerMk ::
+    private toUSize : USize
+  deriving DecidableEq, Hashable
+
+/-- Returns the address of a Lean object. -/
+@[inline] unsafe def addrUnsafe (a : α) : Addr :=
+  ⟨ptrAddrUnsafe a⟩
+
+namespace Addr
+
+noncomputable def mk (a : USize) : Addr :=
+  innerMk a
+
+/-- The null pointer address. The preferred spelling is `0`. -/
+def null : Addr := ⟨0⟩
+
+instance : OfNat Addr 0 := ⟨null⟩
+
+theorem null_eq_zero : null = 0 := rfl
+
+instance : Inhabited Addr := ⟨0⟩
+
+/-- Whether this is a possible address of a Lean object pointer. -/
+def isNonScalar (a : Addr) : Bool :=
+  a.toUSize % 2 == 0
+
+@[simp] theorem isNonScalar_null : isNonScalar 0 := by
+  simp [isNonScalar, ← null_eq_zero, null]
+
+@[inline] def toNat (a : Addr) : Nat :=
+  a.toUSize.toNat
+
+@[simp] theorem toNat_mk : toNat (mk a) = a.toNat := rfl
+
+theorem toNat_inj : toNat a = toNat b ↔ a = b := by
+  cases a; cases b; simp [toNat, ← USize.toNat_inj]
+
+theorem isNonScalar_iff : isNonScalar a ↔ a.toNat % 2 = 0 := by
+  simp [isNonScalar, ← USize.toNat_inj, toNat]
+
+@[inline] def toUInt64 (a : Addr) : UInt64 :=
+  a.toUSize.toUInt64
+
+@[simp] theorem toNat_toUInt64 : (toUInt64 a).toNat = a.toNat := rfl
